Try reformulating translation more simply, WIP
Rebased on more automated proofs on master, which stay mostly the same after
these changes.

theories/AAsynToSem.v
@@ -1,4 +1,6 @@
 (** Define translation from syntactic terms/values to semantic ones, following Sec. 3.2 of the PDF. *)
+From iris.proofmode Require Import tactics.
+From iris.program_logic Require Import ectx_lifting.
 From Dot Require Import tactics synFuncs operational.
 From iris.proofmode Require Import tactics.
 From iris.program_logic Require Import ectx_lifting.
@@ -7,6 +9,10 @@ Import operational.lang.
 Section Sec.
   Context `{HdotG: dotG Σ}.
   Context `{dotInterpG Σ}.
+
+  Lemma alloc_sp T:
+    (|==> ∃ γ, γ ⤇ dot_interp T)%I.
+  Proof. by apply saved_interp_alloc. Qed.
 
   (** We define the translation relation T between syntactic and semantic
       values, terms, types, and so on.
@@ -20,275 +26,370 @@ Section Sec.
 
   (** Translation between syntactic and semantic *type member definitions*.
     This is the interesting case of the translation. *)
-  Definition t_dty_syn2sem (t_ty: vls -> ty -> ty -> iProp Σ) (T1: ty) (σ σ2: vls) γ2: iProp Σ :=
-    (∃ φ T2, γ2 ⤇ φ ∧ t_ty σ T1 T2 ∧
+  Definition is_stamped_dty (T: ty) (σ: vls) γ: iProp Σ :=
+    (∃ φ, γ ⤇ φ ∧
              ∀ ρ v,
+               ⌜ length ρ = length σ ⌝ →
                (* We should demand that ρ is closed, and we should check that FV (T) ⊂ dom σ *)
-               dot_interp T2 (subst_sigma σ ρ) v ≡ φ (subst_sigma σ2 ρ) v)%I.
+               dot_interp T ρ v ≡ φ (subst_sigma σ ρ) v)%I.
+  Instance is_stamped_dty_persistent T σ γ: Persistent (is_stamped_dty T σ γ).
+  Proof. apply _. Qed.
 
   (** Lift translation between syntactic and semantic entities throughout the whole language.
       Lift [t_dty_syn2sem] throughout the syntax of terms and types, checking that otherwise the terms are equal.
    *)
 
-  Fixpoint t_tm (σ: vls) (t1 t2: tm) {struct t1}: iProp Σ :=
-    match (t1, t2) with
-    | (tv v1, tv v2) => t_vl σ v1 v2
-    | (tapp t11 t12, tapp t21 t22) =>
-      t_tm σ t11 t21 ∧ t_tm σ t12 t22
-    | (tproj t1 l1, tproj t2 l2) =>
-      t_tm σ t1 t2 ∧ ⌜l1 = l2⌝
-    | (tskip t1, tskip t2) =>
-      t_tm σ t1 t2
-    | _ => False
-    end%I
-  with
-  t_vl (σ: vls) (v1 v2: vl) {struct v1}: iProp Σ :=
-    match (v1, v2) with
-    | (var_vl i1, var_vl i2) => ⌜i1 = i2⌝
-    | (vabs t1, vabs t2) => t_tm (push_var σ) t1 t2
-    | (vobj ds1, vobj ds2) =>
-      let fix t_dms (σ: vls) (ds1 ds2: dms) : iProp Σ :=
-          (* ([∗ list] d1 ; d2 ∈ ds1 ; ds2 , t_dm σ d1 d2)%I *)
-          match (ds1, ds2) with
-          | (nil, nil) => True
-          | (cons d1 ds1, cons d2 ds2) =>
-            t_dm σ d1 d2 ∧ t_dms σ ds1 ds2
-          | _ => False
-          end%I
-      in
-      t_dms (push_var σ) ds1 ds2
-    | (vnat n1, vnat n2) => ⌜ n1 = n2 ⌝
-    | _ => False
-    end%I
-  with
-  t_dm (σ: vls) (d1 d2: dm) {struct d1}: iProp Σ :=
-    match (d1, d2) with
-    | (dtysyn T1, dtysem σ2 γ2) =>
-      (* Only nontrivial case *)
-      t_dty_syn2sem t_ty T1 σ σ2 γ2
-    | (dvl v1, dvl v2) => t_vl σ v1 v2
-    | _ => False
-    end%I
-  with
-  t_path (σ: vls) (p1 p2: path) {struct p1}: iProp Σ :=
-    match (p1, p2) with
-    | (pv v1, pv v2) => t_vl σ v1 v2
-    | (pself p1 l1, pself p2 l2) => t_path σ p1 p2 ∧ ⌜l1 = l2⌝
-    | _ => False
-    end%I
-  with
-  t_ty (σ: vls) (T1 T2: ty) {struct T1}: iProp Σ :=
-    match (T1, T2) with
-    | (TTop, TTop) => True
-    | (TBot, TBot) => True
-    | (TAnd T11 T12, TAnd T21 T22) =>
-      t_ty σ T11 T21 ∧ t_ty σ T12 T22
-    | (TOr T11 T12, TOr T21 T22) =>
-      t_ty σ T11 T21 ∧ t_ty σ T12 T22
-    | (TLater T1, TLater T2) =>
-      t_ty σ T1 T2
-    | (TAll T11 T12, TAll T21 T22) =>
-      t_ty σ T11 T21 ∧ t_ty (push_var σ) T12 T22
-    | (TMu T1, TMu T2) =>
-      t_ty (push_var σ) T1 T2
-    | (TVMem l1 T1, TVMem l2 T2) => ⌜l1 = l2⌝ ∧ t_ty σ T1 T2
-    | (TTMem l1 T11 T12, TTMem l2 T21 T22) => ⌜l1 = l2⌝ ∧ t_ty σ T11 T21 ∧ t_ty σ T12 T22
-    | (TSel p1 l1, TSel p2 l2) => t_path σ p1 p2 ∧ ⌜l1 = l2⌝
-    | (TSelA p1 l1 T11 T12, TSelA p2 l2 T21 T22) => t_path σ p1 p2 ∧ ⌜l1 = l2⌝ ∧ t_ty σ T11 T21 ∧ t_ty σ T12 T22
-    | (TNat, TNat) => True
-    | _ => False
-    end%I
-  .
-
-  (** Translation for definitions. Used? *)
-  Definition t_dms (σ: vls) (ds1 ds2: dms) : iProp Σ :=
-    ([∗ list] d1 ; d2 ∈ ds1 ; ds2 , t_dm σ d1 d2)%I.
-  Global Arguments t_dms _ /.
-  (** Translation for value sequences [vls]. Probably unused. *)
-  Definition t_vls (σ: vls) (vs1 vs2: vls) : iProp Σ :=
-    ([∗ list] v1 ; v2 ∈ vs1 ; vs2 , t_vl σ v1 v2)%I.
-
-  (** For each type T, we can save its interpretation in the ghost state.
-      Caveat: you only want to use this on translated (semantic) types. Not to
-      be confused with the results of the interpretation (ARGH).
-   *)
-  Lemma alloc_sp T:
-    (|==> ∃ γ, γ ⤇ dot_interp T)%I.
-  Proof. by apply saved_interp_alloc. Qed.
-
-  (** The translation relation is persistent. *)
-  Lemma t_ty_persistent t1 t2 σ: Persistent (t_ty σ t1 t2)
-  with  t_path_persistent t1 t2 σ: Persistent (t_path σ t1 t2)
-  with  t_vl_persistent t1 t2 σ: Persistent (t_vl σ t1 t2)
-  with  t_tm_persistent t1 t2 σ: Persistent (t_tm σ t1 t2)
-  with  t_dm_persistent t1 t2 σ: Persistent (t_dm σ t1 t2).
-  Proof.
-    all: revert t1 t2 σ; induction t1; destruct t2;
-      try (revert l0; induction l; destruct l0);
-      simpl; try apply _.
-  Qed.
-  Global Existing Instance t_ty_persistent.
-  Global Existing Instance t_path_persistent.
-  Global Existing Instance t_vl_persistent.
-  Global Existing Instance t_tm_persistent.
-  Global Existing Instance t_dm_persistent.
-
-  Lemma t_dms_persistent ds1 ds2 σ: Persistent (t_dms σ ds1 ds2).
-  Proof.
-    revert ds1 ds2 σ; induction ds1; destruct ds2; simpl;
-      try apply _.
-  Qed.
-  Global Existing Instance t_dms_persistent.
-
-  (** We now prove the lemmas on *existence of translations*, in stages.
-      FIXME: unlike on paper, we do not yet check free variables.
-   *)
-
-  (** Existence of translations for type member definitions. *)
-  Lemma ex_t_dty T1 T2 σ:
-    t_ty σ T1 T2 -∗
-    (|==> ∃(d: dm), t_dm σ (dtysyn T1) d)%I.
-  Proof.
-    iMod (alloc_sp T2) as (γ) "#Hγ".
-    iIntros "#HT !> /=".
-    rewrite /t_dty_syn2sem.
-    by iExists (dtysem σ γ), (dot_interp T2), T2; repeat iSplit.
-  Qed.
-
-  (** is_syn_* are predicates to distinguish syntactic entities/source syntax.
+  (** is_stamped_* are predicates to distinguish syntactic entities/source syntax.
       They also check for free variables at the same time, but that's probably a bad idea.
    *)
-  Fixpoint is_syn_tm (n: nat) (t: tm): Prop :=
+  Fixpoint is_stamped_tm (t: tm): iProp Σ :=
     match t with
     | tv v =>
-      is_syn_vl n v
+      is_stamped_vl v
     | tapp t1 t2 =>
-      is_syn_tm n t1 ∧ is_syn_tm n t2
+      is_stamped_tm t1 ∧ is_stamped_tm t2
     | tproj t l =>
-      is_syn_tm n t
+      is_stamped_tm t
     | tskip t =>
-      is_syn_tm n t
-    end
+      is_stamped_tm t
+    end%I
   with
-  is_syn_vl (n: nat) (v1: vl): Prop :=
+  is_stamped_vl (v1: vl): iProp Σ :=
     match v1 with
-    | var_vl i => i < n
-    | vabs t => is_syn_tm (S n) t
+    | var_vl i => True
+    | vabs t => is_stamped_tm t
     | vobj ds =>
-      let fix is_syn_dms (n: nat) (ds: dms): Prop :=
+      let fix is_stamped_dms (ds: dms): iProp Σ :=
           match ds with
-          | nil => True
-          | cons d ds =>
-            is_syn_dm n d ∧ is_syn_dms n ds
+          | [] => True
+          | d :: ds =>
+            is_stamped_dm d ∧ is_stamped_dms ds
           end
         in
-          is_syn_dms (S n) ds
-    | vnat n => True
-    end
+          is_stamped_dms ds
+    | vnat _ => True
+    end%I
   with
-  is_syn_dm (n: nat) (d: dm): Prop :=
+  is_stamped_dm (d: dm): iProp Σ :=
     match d with
     (* Only nontrivial case *)
-    | dtysyn T =>
-      is_syn_ty n T
-    | dtysem _ _ => False
-    | dvl v1 => is_syn_vl n v1
-    end
+    | dty T σ (Some γ) =>
+      let fix is_stamped_vls (vs: vls): iProp Σ :=
+          match vs with
+          | [] => True
+          | v :: vs =>
+            is_stamped_vl v ∧ is_stamped_vls vs
+          end
+      in
+      is_stamped_ty T ∧
+      is_stamped_vls σ ∧
+      is_stamped_dty T σ γ
+    | dty T σ None => False
+    | dvl v1 => is_stamped_vl v1
+    end%I
   with
-  is_syn_path (n: nat) (p1: path): Prop :=
+  is_stamped_path (p1: path): iProp Σ :=
     match p1 with
-    | pv v => is_syn_vl n v
-    | pself p l => is_syn_path n p
-    end
+    | pv v => is_stamped_vl v
+    | pself p l => is_stamped_path p
+    end%I
   with
-  is_syn_ty (n: nat) (T1: ty): Prop :=
+  is_stamped_ty (T1: ty): iProp Σ :=
     match T1 with
     | TTop => True
     | TBot => True
     | TAnd T1 T2 =>
-      is_syn_ty n T1 ∧ is_syn_ty n T2
+      is_stamped_ty T1 ∧ is_stamped_ty T2
     | TOr T1 T2 =>
-      is_syn_ty n T1 ∧ is_syn_ty n T2
+      is_stamped_ty T1 ∧ is_stamped_ty T2
     | TLater T1 =>
-      is_syn_ty n T1
+      is_stamped_ty T1
     | TAll T1 T2 =>
-      is_syn_ty n T1 ∧ is_syn_ty (S n) T2
+      is_stamped_ty T1 ∧ is_stamped_ty T2
     | TMu T =>
-      is_syn_ty (S n) T
-    | TVMem l T => is_syn_ty n T
-    | TTMem l T1 T2 => is_syn_ty n T1 ∧ is_syn_ty n T2
-    | TSel p l => is_syn_path n p
-    | TSelA p l T1 T2 => is_syn_path n p ∧ is_syn_ty n T1 ∧ is_syn_ty n T2
+      is_stamped_ty T
+    | TVMem l T => is_stamped_ty T
+    | TTMem l T1 T2 => is_stamped_ty T1 ∧ is_stamped_ty T2
+    | TSel p l => is_stamped_path p
+    | TSelA p l T1 T2 => is_stamped_path p ∧ is_stamped_ty T1 ∧ is_stamped_ty T2
     | TNat => True
-    end.
+    end%I.
 
-  Definition is_syn_dms (n: nat) (ds: dms): Prop :=
-    Forall (is_syn_dm n) ds.
+  (** For each type T, we can save its interpretation in the ghost state. *)
+  (*     Caveat: you only want to use this on translated (semantic) types. Not to *)
+  (*     be confused with the results of the interpretation (ARGH). *)
+  (*  *)
+  (** The translation relation is persistent. *)
 
-  Ltac iModSpec H xt :=
-    iMod H as (xt) "#?"; try intuition eassumption.
-
-  Ltac pickSigmaInHp :=
-    cbn; repeat match goal with
-                  | H : context [?p _ ?t1 ] |- context [?p ?σ ?t1 _] =>
-                    let x := fresh "TEMP" in
-                    evar (x:nat);
-                    specialize (H σ x); subst x;
-                    let xt := fresh "t" in
-                    iModSpec H xt
-                  end.
-
-  Tactic Notation "finish" uconstr(p) := iIntros "!>"; iExists p; simpl; repeat iSplit; auto.
-  Tactic Notation "recursiveTransf" uconstr(p) := pickSigmaInHp; finish p.
-  Ltac fill :=
-    lazymatch goal with
-    | |- context [(∃ t2, ?p ?σ (?c ?t11 ?t12) t2)%I] =>
-      recursiveTransf (c _ _)
-    | |- context [(∃ t2, ?p ?σ (?c ?t11) t2)%I] =>
-      recursiveTransf (c _)
-    | |- context [(∃ t2, ?p ?σ ?c t2)%I] =>
-      recursiveTransf c
-    end.
-  Ltac skeleton σ n t1 := revert σ n; induction t1; intros * Hsyn; simpl in Hsyn; try solve [contradiction|fill].
-
-  (** BEWARE!
-   Not using Admitted here, as it skips well-foundedness checks, which are
-   important here. **)
-  Axiom false: False.
-  Ltac skipAdmit := exfalso; apply false.
-
-  Lemma ex_t_ty σ n t1: is_syn_ty n t1 -> (|==> ∃t2, t_ty σ t1 t2)%I
-  with  ex_t_path σ n t1: is_syn_path n t1 -> (|==> ∃t2, t_path σ t1 t2)%I
-  with  ex_t_vl σ n t1: is_syn_vl n t1 -> (|==> ∃t2, t_vl σ t1 t2)%I
-  with  ex_t_tm σ n t1: is_syn_tm n t1 -> (|==> ∃t2, t_tm σ t1 t2)%I
-  with  ex_t_dm σ n t1: is_syn_dm n t1 -> (|==> ∃t2, t_dm σ t1 t2)%I.
-  (* with  ex_t_dms σ n t1: is_syn_dms n t1 -> (|==> ∃t2, t_dms σ t1 t2)%I. *)
+  Lemma is_stamped_ty_persistent t: Persistent (is_stamped_ty t)
+  with  is_stamped_path_persistent t: Persistent (is_stamped_path t)
+  with  is_stamped_vl_persistent t: Persistent (is_stamped_vl t)
+  with  is_stamped_tm_persistent t: Persistent (is_stamped_tm t)
+  with  is_stamped_dm_persistent t: Persistent (is_stamped_dm t).
   Proof.
-    - skeleton σ n t1.
-      + iModSpec (ex_t_path σ n p) p2. finish (TSel _ _).
-      + iModSpec (ex_t_path σ n p) p2. recursiveTransf (TSelA _ _ _ _).
-    - skeleton σ n t1.
-      + iModSpec (ex_t_vl σ n v) v2. finish (pv _).
-    - skeleton σ n t1.
-      + iModSpec (ex_t_tm (push_var σ) (S n) t) t2. finish (vabs _).
-      +
-        (* iModSpec (ex_t_dms (push_var σ) (S n) d) d2. finish (vobj _). *)
-        iInduction l as [|d ds] "IHl".
-        * by iExists (vobj []).
-        * ev.
-          iMod (ex_t_dm (push_var σ) (S n) d H0) as (d2) "#Hd".
-          iMod ("IHl" $! H1) as (v2) "#Hds". iClear "IHl".
-          destruct v2 as [ | | | ds2]; try done.
-          iExists (vobj (d2 :: ds2)).
-          iModIntro; by iSplit.
-    - skeleton σ n t1.
-      + iModSpec (ex_t_vl σ n v) v2. finish (tv _).
-    - skeleton σ n t1.
-      + iModSpec (ex_t_ty σ n t) t2. by iApply ex_t_dty.
-      + iModSpec (ex_t_vl σ n v) v2. finish (dvl _).
-    (* - skeleton σ n t1. *)
-    (*   + iModSpec (ex_t_dm σ n a) d2. recursiveTransf (cons _ _). *)
+    all:
+      induction t; simpl;
+      try case_match;
+      (* For the dty case, get to is_stamped_vls before induction or the IH will
+         have the wrong shpe *)
+      repeat apply bi.and_persistent;
+      try induction l; try apply _.
   Qed.
+  Global Existing Instance is_stamped_ty_persistent.
+  Global Existing Instance is_stamped_path_persistent.
+  Global Existing Instance is_stamped_vl_persistent.
+  Global Existing Instance is_stamped_tm_persistent.
+  Global Existing Instance is_stamped_dm_persistent.
+
+
+  (* Fixpoint t_tm (σ: vls) (t1 t2: tm) {struct t1}: iProp Σ := *)
+  (*   match (t1, t2) with *)
+  (*   | (tv v1, tv v2) => t_vl σ v1 v2 *)
+  (*   | (tapp t11 t12, tapp t21 t22) => *)
+  (*     t_tm σ t11 t21 ∧ t_tm σ t12 t22 *)
+  (*   | (tproj t1 l1, tproj t2 l2) => *)
+  (*     t_tm σ t1 t2 ∧ ⌜l1 = l2⌝ *)
+  (*   | (tskip t1, tskip t2) => *)
+  (*     t_tm σ t1 t2 *)
+  (*   | _ => False *)
+  (*   end%I *)
+  (* with *)
+  (* t_vl (σ: vls) (v1 v2: vl) {struct v1}: iProp Σ := *)
+  (*   match (v1, v2) with *)
+  (*   | (var_vl i1, var_vl i2) => ⌜i1 = i2⌝ *)
+  (*   | (vabs t1, vabs t2) => t_tm (push_var σ) t1 t2 *)
+  (*   | (vobj ds1, vobj ds2) => *)
+  (*     let fix t_dms (σ: vls) (ds1 ds2: dms) : iProp Σ := *)
+  (*         (* ([∗ list] d1 ; d2 ∈ ds1 ; ds2 , t_dm σ d1 d2)%I *) *)
+  (*         match (ds1, ds2) with *)
+  (*         | (nil, nil) => True *)
+  (*         | (cons d1 ds1, cons d2 ds2) => *)
+  (*           t_dm σ d1 d2 ∧ t_dms σ ds1 ds2 *)
+  (*         | _ => False *)
+  (*         end%I *)
+  (*     in *)
+  (*     t_dms (push_var σ) ds1 ds2 *)
+  (*   | (vnat n1, vnat n2) => ⌜ n1 = n2 ⌝ *)
+  (*   | _ => False *)
+  (*   end%I *)
+  (* with *)
+  (* t_dm (σ: vls) (d1 d2: dm) {struct d1}: iProp Σ := *)
+  (*   match (d1, d2) with *)
+  (*   | (dtysyn T1, dtysem σ2 γ2) => *)
+  (*     (* Only nontrivial case *) *)
+  (*     t_dty_syn2sem t_ty T1 σ σ2 γ2 *)
+  (*   | (dvl v1, dvl v2) => t_vl σ v1 v2 *)
+  (*   | _ => False *)
+  (*   end%I *)
+  (* with *)
+  (* t_path (σ: vls) (p1 p2: path) {struct p1}: iProp Σ := *)
+  (*   match (p1, p2) with *)
+  (*   | (pv v1, pv v2) => t_vl σ v1 v2 *)
+  (*   | (pself p1 l1, pself p2 l2) => t_path σ p1 p2 ∧ ⌜l1 = l2⌝ *)
+  (*   | _ => False *)
+  (*   end%I *)
+  (* with *)
+  (* t_ty (σ: vls) (T1 T2: ty) {struct T1}: iProp Σ := *)
+  (*   match (T1, T2) with *)
+  (*   | (TTop, TTop) => True *)
+  (*   | (TBot, TBot) => True *)
+  (*   | (TAnd T11 T12, TAnd T21 T22) => *)
+  (*     t_ty σ T11 T21 ∧ t_ty σ T12 T22 *)
+  (*   | (TOr T11 T12, TOr T21 T22) => *)
+  (*     t_ty σ T11 T21 ∧ t_ty σ T12 T22 *)
+  (*   | (TLater T1, TLater T2) => *)
+  (*     t_ty σ T1 T2 *)
+  (*   | (TAll T11 T12, TAll T21 T22) => *)
+  (*     t_ty σ T11 T21 ∧ t_ty (push_var σ) T12 T22 *)
+  (*   | (TMu T1, TMu T2) => *)
+  (*     t_ty (push_var σ) T1 T2 *)
+  (*   | (TVMem l1 T1, TVMem l2 T2) => ⌜l1 = l2⌝ ∧ t_ty σ T1 T2 *)
+  (*   | (TTMem l1 T11 T12, TTMem l2 T21 T22) => ⌜l1 = l2⌝ ∧ t_ty σ T11 T21 ∧ t_ty σ T12 T22 *)
+  (*   | (TSel p1 l1, TSel p2 l2) => t_path σ p1 p2 ∧ ⌜l1 = l2⌝ *)
+  (*   | (TSelA p1 l1 T11 T12, TSelA p2 l2 T21 T22) => t_path σ p1 p2 ∧ ⌜l1 = l2⌝ ∧ t_ty σ T11 T21 ∧ t_ty σ T12 T22 *)
+  (*   | (TNat, TNat) => True *)
+  (*   | _ => False *)
+  (*   end%I *)
+  (* . *)
+
+  (* (** Translation for definitions. Used? *) *)
+  (* Definition t_dms (σ: vls) (ds1 ds2: dms) : iProp Σ := *)
+  (*   ([ list] d1 ; d2 ∈ ds1 ; ds2 , t_dm σ d1 d2)%I. *)
+  (* Global Arguments t_dms _ /. *)
+  (* (** Translation for value sequences [vls]. Probably unused. *) *)
+  (* Definition t_vls (σ: vls) (vs1 vs2: vls) : iProp Σ := *)
+  (*   ([∗ list] v1 ; v2 ∈ vs1 ; vs2 , t_vl σ v1 v2)%I. *)
+
+  (* (** For each type T, we can save its interpretation in the ghost state. *)
+  (*     Caveat: you only want to use this on translated (semantic) types. Not to *)
+  (*     be confused with the results of the interpretation (ARGH). *)
+  (*  *) *)
+  (* (** The translation relation is persistent. *) *)
+  (* Lemma t_ty_persistent t1 t2 σ: Persistent (t_ty σ t1 t2) *)
+  (* with  t_path_persistent t1 t2 σ: Persistent (t_path σ t1 t2) *)
+  (* with  t_vl_persistent t1 t2 σ: Persistent (t_vl σ t1 t2) *)
+  (* with  t_tm_persistent t1 t2 σ: Persistent (t_tm σ t1 t2) *)
+  (* with  t_dm_persistent t1 t2 σ: Persistent (t_dm σ t1 t2). *)
+  (* Proof. *)
+  (*   all: revert t1 t2 σ; induction t1; destruct t2; *)
+  (*     try (revert l0; induction l; destruct l0); *)
+  (*     simpl; try apply _. *)
+  (* Qed. *)
+  (* Global Existing Instance t_ty_persistent. *)
+  (* Global Existing Instance t_path_persistent. *)
+  (* Global Existing Instance t_vl_persistent. *)
+  (* Global Existing Instance t_tm_persistent. *)
+  (* Global Existing Instance t_dm_persistent. *)
+
+  (* Lemma t_dms_persistent ds1 ds2 σ: Persistent (t_dms σ ds1 ds2). *)
+  (* Proof. *)
+  (*   revert ds1 ds2 σ; induction ds1; destruct ds2; simpl; *)
+  (*     try apply _. *)
+  (* Qed. *)
+  (* Global Existing Instance t_dms_persistent. *)
+
+  (** We now prove the lemmas on *existence of translations*, in stages.
+      FIXME: unlike on paper, we do not yet check free variables.
+   *)
+  Implicit Types
+           (L T U: ty) (v: vl) (e: tm) (d: dm) (ds: dms)
+           (Γ : ctx) (ρ : leibnizC vls).
+
+  (* Definition of fv_n for values must use subst not hsubst. *)
+  Definition fv_n_vl (v: vl) n :=
+    ∀ s1 s2, (∀ x, x < n → s1 x = s2 x) → v.[s1] = v.[s2].
+
+  Definition fv_n `{HSubst vl X} (t: X) n :=
+    ∀ s1 s2, (∀ x, x < n → s1 x = s2 x) → t.|[s1] = t.|[s2].
+
+  Fixpoint idsσ n: vls :=
+    match n with
+    | 0 => []
+    | S n => push_var (idsσ n)
+    end.
+
+  Lemma length_idsσr n r: length (idsσ n).|[ren r] = n.
+  Proof.
+    elim : n r => [r | n IHn r] => //.
+    asimpl. by rewrite IHn.
+  Qed.
+
+  Lemma length_idsσ n: length (idsσ n) = n.
+  Proof. pose proof (length_idsσr n (+0)) as Hr. asimpl in Hr. exact Hr. Qed.
+
+  Lemma subst_sigma_idsσ ρ n : length ρ = n →
+                  (subst_sigma (idsσ n) ρ) ≡ ρ.
+  Proof.
+    rewrite /subst_sigma. move :n.
+    induction ρ => *; subst => //; asimpl.
+    f_equal. by apply IHρ.
+  Qed.
+
+  Lemma is_stamped_var i: is_stamped_vl (var_vl i).
+  Proof. by []. Qed.
+
+  Definition is_stamped_vls :=
+    (fix is_stamped_vls (vs: vls): iProp Σ :=
+       match vs with
+       | [] => True
+       | v :: vs =>
+         is_stamped_vl v ∧ is_stamped_vls vs
+       end%I).
+
+  Lemma is_stamped_vls_idsσr n r:
+    is_stamped_vls ((idsσ n).|[ren r]).
+  Proof.
+    iInduction n as [ | ] "IHn" forall (r); first trivial.
+    asimpl; iSplit; trivial.
+  Qed.
+
+  Lemma is_stamped_vls_idsσ n: is_stamped_vls (idsσ n).
+  Proof. pose proof (is_stamped_vls_idsσr n (+0)) as Hr. asimpl in Hr. exact Hr. Qed.
+
+  (** Existence of translations for type member definitions. *)
+  Lemma ex_t_dty T n:
+    fv_n T n →
+    is_stamped_ty T -∗
+    (|==> ∃ σ γ, is_stamped_dm (dty T σ (Some γ)))%I.
+  Proof.
+    intros Hfv. iMod (alloc_sp T) as (γ) "#Hγ".
+    iIntros "#HT !> /=".
+    iExists (idsσ n), γ; repeat iSplit; try done.
+    - iApply is_stamped_vls_idsσ.
+    - rewrite /is_stamped_dty.
+      iExists (dot_interp T); repeat iSplit; try done.
+      rewrite length_idsσ. iIntros. by rewrite (subst_sigma_idsσ ρ n).
+  Qed.
+
+  (* (** is_syn_* are predicates to distinguish syntactic entities/source syntax. *)
+  (*     They also check for free variables at the same time, but that's probably a bad idea. *)
+  (*  *) *)
+  (* Fixpoint is_syn_tm (n: nat) (t: tm): Prop := *)
+  (*   match t with *)
+  (*   | tv v => *)
+  (*     is_syn_vl n v *)
+  (*   | tapp t1 t2 => *)
+  (*     is_syn_tm n t1 ∧ is_syn_tm n t2 *)
+  (*   | tproj t l => *)
+  (*     is_syn_tm n t *)
+  (*   | tskip t => *)
+  (*     is_syn_tm n t *)
+  (*   end *)
+  (* with *)
+  (* is_syn_vl (n: nat) (v1: vl): Prop := *)
+  (*   match v1 with *)
+  (*   | var_vl i => i < n *)
+  (*   | vabs t => is_syn_tm (S n) t *)
+  (*   | vobj ds => *)
+  (*     let fix is_syn_dms (n: nat) (ds: dms): Prop := *)
+  (*         match ds with *)
+  (*         | nil => True *)
+  (*         | cons d ds => *)
+  (*           is_syn_dm n d ∧ is_syn_dms n ds *)
+  (*         end *)
+  (*       in *)
+  (*         is_syn_dms (S n) ds *)
+  (*   | vnat n => True *)
+  (*   end *)
+  (* with *)
+  (* is_syn_dm (n: nat) (d: dm): Prop := *)
+  (*   match d with *)
+  (*   (* Only nontrivial case *) *)
+  (*   | dtysyn T => *)
+  (*     is_syn_ty n T *)
+  (*   | dtysem _ _ => False *)
+  (*   | dvl v1 => is_syn_vl n v1 *)
+  (*   end *)
+  (* with *)
+  (* is_syn_path (n: nat) (p1: path): Prop := *)
+  (*   match p1 with *)
+  (*   | pv v => is_syn_vl n v *)
+  (*   | pself p l => is_syn_path n p *)
+  (*   end *)
+  (* with *)
+  (* is_syn_ty (n: nat) (T1: ty): Prop := *)
+  (*   match T1 with *)
+  (*   | TTop => True *)
+  (*   | TBot => True *)
+  (*   | TAnd T1 T2 => *)
+  (*     is_syn_ty n T1 ∧ is_syn_ty n T2 *)
+  (*   | TOr T1 T2 => *)
+  (*     is_syn_ty n T1 ∧ is_syn_ty n T2 *)
+  (*   | TLater T1 => *)
+  (*     is_syn_ty n T1 *)
+  (*   | TAll T1 T2 => *)
+  (*     is_syn_ty n T1 ∧ is_syn_ty (S n) T2 *)
+  (*   | TMu T => *)
+  (*     is_syn_ty (S n) T *)
+  (*   | TVMem l T => is_syn_ty n T *)
+  (*   | TTMem l T1 T2 => is_syn_ty n T1 ∧ is_syn_ty n T2 *)
+  (*   | TSel p l => is_syn_path n p *)
+  (*   | TSelA p l T1 T2 => is_syn_path n p ∧ is_syn_ty n T1 ∧ is_syn_ty n T2 *)
+  (*   | TNat => True *)
+  (*   end. *)
+
+  (* Definition is_syn_dms (n: nat) (ds: dms): Prop := *)
+  (*   Forall (is_syn_dm n) ds. *)
 
   Fixpoint same_skel_tm (t1 t2: tm): Prop :=
     match (t1, t2) with
@@ -321,19 +422,19 @@ Section Sec.
   with
   same_skel_dm (d1 d2: dm): Prop :=
     match (d1, d2) with
-    | (dtysyn T1, dtysem σ2 γ2) =>
+    | (dty T1 _ _, dty T2 _ _) =>
       (* Only nontrivial case *)
-      True
+      same_skel_ty T1 T2
     | (dvl v1, dvl v2) => same_skel_vl v1 v2
     | _ => False
-    end.
-  Fixpoint same_skel_path (p1 p2: path): Prop :=
+    end
+  with same_skel_path (p1 p2: path): Prop :=
     match (p1, p2) with
     | (pv v1, pv v2) => same_skel_vl v1 v2
     | (pself p1 l1, pself p2 l2) => same_skel_path p1 p2 ∧ l1 = l2
     | _ => False
-    end.
-  Fixpoint same_skel_ty (T1 T2: ty): Prop :=
+    end
+  with same_skel_ty (T1 T2: ty): Prop :=
     match (T1, T2) with
     | (TTop, TTop) => True
     | (TBot, TBot) => True
@@ -355,37 +456,106 @@ Section Sec.
     | _ => False
     end.
 
-  Lemma translation_same_skel σ t t':
-    ( t_tm σ t t' → ⌜same_skel_tm t t'⌝)%I
-  with translation_same_ty σ t t':
-    ( t_ty σ t t' → ⌜same_skel_ty t t'⌝)%I
-  with translation_same_path σ t t':
-    ( t_path σ t t' → ⌜same_skel_path t t'⌝)%I
-  with translation_same_dm σ t t':
-    ( t_dm σ t t' → ⌜same_skel_dm t t'⌝)%I
-  (* with translation_same_skel_dms σ t t': *)
-  (*   ( t_dms σ t t' → ⌜same_skel_dms t t'⌝)%I *)
-  with translation_same_skel_vl σ t t':
-    ( t_vl σ t t' → ⌜same_skel_vl t t'⌝)%I.
-  Proof.
-    Ltac localAuto :=
-      match goal with
-      | [ HH: context[?P _ _ _] |- context[?P _ _ _] ] => iApply HH; try done
-      | _ => try done
-      end.
-    all: iIntros "Hyp";
-      destruct t; destruct t'; simpl; eauto;
-      (* by iApply translation_same_skel_vl. *)
-      repeat iSplit;
-      try (iDestruct "Hyp" as "[Hyp1 Hyp2]");
-      try (iDestruct "Hyp1" as "[Hyp11 Hyp12]");
-      try (iDestruct "Hyp2" as "[Hyp21 Hyp22]");
-      try (iDestruct "Hyp22" as "[Hyp221 Hyp222]"); localAuto.
-    iInduction l as [| d l] "IHl" forall (l0); destruct l0 as [|d0 l0]; try done.
-    repeat iSplit;
-      try (iDestruct "Hyp" as "[Hyp1 Hyp2]"); localAuto.
-    by iApply "IHl".
-  Qed.
+  (* Next, prove existence of stamped terms that share skeletons and type *)
+  (* members with original terms. We need not check if the original terms work. *)
+
+  (* Ltac iModSpec H xt := *)
+  (*   iMod H as (xt) "#?"; try intuition eassumption. *)
+
+  (* Ltac pickSigmaInHp := *)
+  (*   cbn; repeat match goal with *)
+  (*                 | H : context [?p _ ?t1 ] |- context [?p ?σ ?t1 _] => *)
+  (*                   let x := fresh "TEMP" in *)
+  (*                   evar (x:nat); *)
+  (*                   specialize (H σ x); subst x; *)
+  (*                   let xt := fresh "t" in *)
+  (*                   iModSpec H xt *)
+  (*                 end. *)
+
+  (* Tactic Notation "finish" uconstr(p) := iIntros "!>"; iExists p; simpl; repeat iSplit; auto. *)
+  (* Tactic Notation "recursiveTransf" uconstr(p) := pickSigmaInHp; finish p. *)
+  (* Ltac fill := *)
+  (*   lazymatch goal with *)
+  (*   | |- context [(∃ t2, ?p ?σ (?c ?t11 ?t12) t2)%I] => *)
+  (*     recursiveTransf (c _ _) *)
+  (*   | |- context [(∃ t2, ?p ?σ (?c ?t11) t2)%I] => *)
+  (*     recursiveTransf (c _) *)
+  (*   | |- context [(∃ t2, ?p ?σ ?c t2)%I] => *)
+  (*     recursiveTransf c *)
+  (*   end. *)
+  (* Ltac skeleton σ n t1 := revert σ n; induction t1; intros * Hsyn; simpl in Hsyn; try solve [contradiction|fill]. *)
+
+  (* (** BEWARE! *)
+  (*  Not using Admitted here, as it skips well-foundedness checks, which are *)
+  (*  important here. **) *)
+  (* Axiom false: False. *)
+  (* Ltac skipAdmit := exfalso; apply false. *)
+
+  (* Lemma ex_t_ty σ n t1: is_syn_ty n t1 -> (|==> ∃t2, t_ty σ t1 t2)%I *)
+  (* with  ex_t_path σ n t1: is_syn_path n t1 -> (|==> ∃t2, t_path σ t1 t2)%I *)
+  (* with  ex_t_vl σ n t1: is_syn_vl n t1 -> (|==> ∃t2, t_vl σ t1 t2)%I *)
+  (* with  ex_t_tm σ n t1: is_syn_tm n t1 -> (|==> ∃t2, t_tm σ t1 t2)%I *)
+  (* with  ex_t_dm σ n t1: is_syn_dm n t1 -> (|==> ∃t2, t_dm σ t1 t2)%I. *)
+  (* (* with  ex_t_dms σ n t1: is_syn_dms n t1 -> (|==> ∃t2, t_dms σ t1 t2)%I. *) *)
+  (* Proof. *)
+  (*   - skeleton σ n t1. *)
+  (*     + iModSpec (ex_t_path σ n p) p2. finish (TSel _ _). *)
+  (*     + iModSpec (ex_t_path σ n p) p2. recursiveTransf (TSelA _ _ _ _). *)
+  (*   - skeleton σ n t1. *)
+  (*     + iModSpec (ex_t_vl σ n v) v2. finish (pv _). *)
+  (*   - skeleton σ n t1. *)
+  (*     + iModSpec (ex_t_tm (push_var σ) (S n) t) t2. finish (vabs _). *)
+  (*     + *)
+  (*       (* iModSpec (ex_t_dms (push_var σ) (S n) d) d2. finish (vobj _). *) *)
+  (*       iInduction l as [|d ds] "IHl". *)
+  (*       * by iExists (vobj []). *)
+  (*       * ev. *)
+  (*         iMod (ex_t_dm (push_var σ) (S n) d H0) as (d2) "#Hd". *)
+  (*         iMod ("IHl" $! H1) as (v2) "#Hds". iClear "IHl". *)
+  (*         destruct v2 as [ | | | ds2]; try done. *)
+  (*         iExists (vobj (d2 :: ds2)). *)
+  (*         iModIntro; by iSplit. *)
+  (*   - skeleton σ n t1. *)
+  (*     + iModSpec (ex_t_vl σ n v) v2. finish (tv _). *)
+  (*   - skeleton σ n t1. *)
+  (*     + iModSpec (ex_t_ty σ n t) t2. by iApply ex_t_dty. *)
+  (*     + iModSpec (ex_t_vl σ n v) v2. finish (dvl _). *)
+  (*   (* - skeleton σ n t1. *) *)
+  (*   (*   + iModSpec (ex_t_dm σ n a) d2. recursiveTransf (cons _ _). *) *)
+  (* Qed. *)
+
+
+  (* Lemma translation_same_skel σ t t': *)
+  (*   ( t_tm σ t t' → ⌜same_skel_tm t t'⌝)%I *)
+  (* with translation_same_ty σ t t': *)
+  (*   ( t_ty σ t t' → ⌜same_skel_ty t t'⌝)%I *)
+  (* with translation_same_path σ t t': *)
+  (*   ( t_path σ t t' → ⌜same_skel_path t t'⌝)%I *)
+  (* with translation_same_dm σ t t': *)
+  (*   ( t_dm σ t t' → ⌜same_skel_dm t t'⌝)%I *)
+  (* (* with translation_same_skel_dms σ t t': *) *)
+  (* (*   ( t_dms σ t t' → ⌜same_skel_dms t t'⌝)%I *) *)
+  (* with translation_same_skel_vl σ t t': *)
+  (*   ( t_vl σ t t' → ⌜same_skel_vl t t'⌝)%I. *)
+  (* Proof. *)
+  (*   Ltac localAuto := *)
+  (*     match goal with *)
+  (*     | [ HH: context[?P _ _ _] |- context[?P _ _ _] ] => iApply HH; try done *)
+  (*     | _ => try done *)
+  (*     end. *)
+  (*   all: iIntros "Hyp"; *)
+  (*     destruct t; destruct t'; simpl; eauto; *)
+  (*     (* by iApply translation_same_skel_vl. *) *)
+  (*     repeat iSplit; *)
+  (*     try (iDestruct "Hyp" as "[Hyp1 Hyp2]"); *)
+  (*     try (iDestruct "Hyp1" as "[Hyp11 Hyp12]"); *)
+  (*     try (iDestruct "Hyp2" as "[Hyp21 Hyp22]"); *)
+  (*     try (iDestruct "Hyp22" as "[Hyp221 Hyp222]"); localAuto. *)
+  (*   iInduction l as [| d l] "IHl" forall (l0); destruct l0 as [|d0 l0]; try done. *)
+  (*   repeat iSplit; *)
+  (*     try (iDestruct "Hyp" as "[Hyp1 Hyp2]"); localAuto. *)
+  (*   by iApply "IHl". *)
+  (* Qed. *)
 
   Fixpoint same_skel_ectx K K' :=
     match K, K' with
@@ -411,11 +581,11 @@ Section Sec.
 
   (* Generalize over all the syntax, and same_skeleton environments. I proved
      same_skel_tm_subst just as a minimal sanity check. *)
-  Lemma same_skel_vl_subst e e' v v':
-    same_skel_vl e e' → same_skel_vl v v' →
-    same_skel_vl (e.[v/]) (e'.[v'/]).
+  Lemma same_skel_vl_subst u u' v v':
+    same_skel_vl u u' → same_skel_vl v v' →
+    same_skel_vl (u.[v/]) (u'.[v'/]).
   Proof.
-    move: e'; induction e; destruct e';
+    move: u'; induction u; destruct u';
     move => Hske Hskv;
       cbn in Hske |- *; try inversion Hske; ev; asimpl; auto.
   Admitted.
